Streams

src/bijection.v
@@ -4,24 +4,51 @@ Require Import Lists.List.
 Import ListNotations.
 
 Require ast.
+Require stream.
 Require encode.
 Require decode.
 
-Definition stream := list bool.
-
-(* Degenerate case *)
-Compute (encode.number 1 9).
-Compute (decode.number 1 [true]).
-
-Lemma number: forall (bits: nat) (n: N) (s s': stream),
-    (N.size_nat n) <= (S bits) ->
-    (decode.number (S bits) s) = Some (n, s')
-    <-> (encode.number (S bits) n) = (firstn (S bits) s).
+Fact positive_size_lt0: forall (p: positive), Pos.size_nat p > 0.
 Proof.
-  induction bits; split; intros.
-  - destruct s.
-    + discriminate.
-    + destruct b; injection H0; intros; subst; trivial.
-  - destruct s.
-    + compute. discriminate.
-    + simpl in H0. destruct b. compute.
+  induction p; simpl; omega.
+Qed.
+
+Definition bijection {A}
+           (dec: stream.bit -> option (A * stream.bit))
+           (enc: A -> stream.bit -> stream.bit)
+           (a: A) :=
+  forall (a: A)(s s': stream.bit),
+    (dec s') = Some (a, s) <-> (enc a s) = s'.
+
+Lemma number: forall (bits: nat) (n: N),
+    (N.size_nat n) <= (S bits) ->
+    bijection (decode.number (S bits)) (encode.number (S bits)) n.
+Proof.
+  unfold bijection, decode.number, decode.number_rec.
+  induction bits; split; intros; destruct s; simpl.
+  - destruct n; try destruct p; try trivial;
+      try (contradict H; simpl; apply gt_not_le;
+           specialize positive_size_lt0 with (p);
+           omega).
+    + case_eq (stream.take s'); intros; rewrite H1 in H0.
+      * destruct p. simpl in H0. admit.
+      * admit.
+    + admit.
+  - admit.
+Admitted.
+
+Lemma condition: forall (c: ast.condition),
+    bijection decode.condition encode.condition c.
+Proof.
+Admitted.
+
+Theorem instruction: forall (i: ast.instruction),
+    bijection decode.instruction encode.instruction i.
+Proof.
+Admitted.
+
+Lemma instructions: forall (ins: ast.instructions) (s: stream.bit),
+    (decode.instructions s) = Some ins
+    <-> (encode.instructions ins stream.empty) = s.
+Proof.
+Admitted.
