src/stream.v
@@ -1,0 +1,77 @@
+Require Import Coq.Arith.Arith.
+Require Import Coq.omega.Omega.
+Require Lists.List.
+
+Inductive t (A: Type) :=
+| stream: list A -> t A.
+
+Definition empty {A} := stream A nil.
+
+Definition length {A} (s: t A): nat :=
+  match s with
+  | stream  _ l => List.length l
+  end.
+
+Definition is_finished {A} (s: t A): bool :=
+  match s with
+  | stream _ nil => true
+  | _ => false
+  end.
+
+Definition take {A} (s: t A): option (A * t A) :=
+  match s with
+  | stream _ l =>
+    match l with
+    | nil => None
+    | cons a l => Some (a, stream _ l)
+    end
+  end.
+
+Lemma take_none_length: forall (A: Type)(s: t A),
+    take s = None -> length s = 0.
+Proof.
+  unfold take, length. intros.
+  destruct s. destruct l.
+  - trivial.
+  - discriminate.
+Qed.
+
+Lemma take_some_length: forall (A: Type)(s s': t A)(r: A),
+    take s = Some (r, s') -> length s = S (length s').
+Proof.
+  unfold take, length. intros.
+  destruct s. destruct s'. destruct l.
+  - discriminate.
+  - injection H. intros. subst. reflexivity.
+Qed.
+
+Definition put {A} (v: A) (s: t A): t A :=
+  match s with
+  | stream _ l => stream _ (cons v l)
+  end.
+
+Lemma put_length: forall (A: Type)(v: A)(s: t A),
+    length (put v s) = S (length s).
+Proof.
+  unfold put, length. intros.
+  destruct s. reflexivity.
+Qed.
+
+Fixpoint put_list {A} (l: list A) (s: t A): t A :=
+  match l with
+  | nil => s
+  | cons a l => put_list l (put a s)
+  end.
+
+Definition puts {A}
+           (f: t A -> t A)
+           (l: list A): Prop :=
+  eq (f empty) (put_list l empty).
+
+Definition bit := t bool.
+
+Module BitNotations.
+  Notation "0" := (false): bit_scope.
+  Notation "1" := (true): bit_scope.
+  Delimit Scope bit_scope with bit.
+End BitNotations.
